thesis/fault-modelling-theory/SimpleMonitorExample.thy
@@ -3,54 +3,72 @@ imports SystemModel ValuedTautology
 begin
 
 datatype FailureVarName = FBattery nat | FMon
-datatype ValueVarName = Mon nat
+datatype ValueVarName = MonIn nat | BatOut nat
+
+primrec valuation :: "ValueVarName \<Rightarrow> (FailureVarName, ValueVarName) ValuesOperand" 
+where
+  "valuation (BatOut m) = VBVExpOp [ 
+      VB (VBBExpUnOp Not (VBBVarOp (FBattery m))) (VBVConstOp (FMNominal 5)),
+      VB (VBBVarOp (FBattery m)) (VBVConstOp (FMFailure Omission))
+    ]"
 
 definition Battery :: "nat \<Rightarrow> (FailureVarName, 'vv) Component" where
   "Battery m \<equiv> (m, ({}, { (1, 
-    map_of [ 
-      (1,(VBBExpUnOp Not (VBBVarOp (FBattery m)), VBVConstOp (FMNominal 5))),
-      (2,(VBBVarOp (FBattery m), VBVConstOp (FMFailure Omission))) 
+    VBVExpOp [ 
+      VB (VBBExpUnOp Not (VBBVarOp (FBattery m))) (VBVConstOp (FMNominal 5)),
+      VB (VBBVarOp (FBattery m)) (VBVConstOp (FMFailure Omission))
     ] ) }))"
 
-definition In :: "ValueVarName \<Rightarrow> ((FailureVarName, ValueVarName) ValuedBoolExp)" where
-  "In x \<equiv> map_of [ (1, (VBBConstOp True, VBVVarOp x)) ]"
-  
-
-definition Monitor :: "nat \<Rightarrow> (((FailureVarName, ValueVarName) ValuedBoolExp) \<Rightarrow> bool) \<Rightarrow> 
+definition Monitor :: "nat \<Rightarrow> (((FailureVarName, ValueVarName) ValuesOperand) \<Rightarrow> bool) \<Rightarrow> 
     (FailureVarName, ValueVarName) Component" where
   "Monitor m P \<equiv> (m, ({
-      (1, In (Mon 1)),
-      (2, In (Mon 2))
+      (1, VBVVarOp (MonIn 1)),
+      (2, VBVVarOp (MonIn 2))
     }, {
-      (1, map_of [
-        (1, (VBBExpBinOp 
-              (op \<and>) 
-              (VBBExpUnOp Not (VBBVarOp FMon))
-              (VBBConstOp (P (In (Mon 1)))), 
-            VBVVarOp (Mon 1))),
-        (2, (VBBExpBinOp 
-              (op \<and>) 
-              (VBBExpUnOp Not (VBBVarOp FMon))
-              (VBBExpUnOp Not (VBBConstOp (P (In (Mon 1))))), 
-            VBVVarOp (Mon 2))),
-        (3, (VBBExpBinOp 
-              (op \<and>) 
-              (VBBVarOp FMon)
-              (VBBConstOp (P (In (Mon 1)))), 
-            VBVVarOp (Mon 2))),
-        (4, (VBBExpBinOp 
-              (op \<and>) 
-              (VBBVarOp FMon)
-              (VBBExpUnOp Not (VBBConstOp (P (In (Mon 1))))), 
-            VBVVarOp (Mon 1)))
+      (1, VBVExpOp [
+        VB 
+          (VBBExpBinOp 
+            (op \<and>) 
+            (VBBExpUnOp Not (VBBVarOp FMon))
+            (VBBConstOp (P (VBVVarOp (MonIn 1)))))
+          (VBVVarOp (MonIn 1)),
+        VB 
+          (VBBExpBinOp 
+            (op \<and>) 
+            (VBBExpUnOp Not (VBBVarOp FMon))
+            (VBBExpUnOp Not (VBBConstOp (P (VBVVarOp (MonIn 1))))))
+          (VBVVarOp (MonIn 2)),
+        VB 
+          (VBBExpBinOp 
+            (op \<and>) 
+            (VBBVarOp FMon)
+            (VBBConstOp (P (VBVVarOp (MonIn 1)))))
+          (VBVVarOp (MonIn 2)),
+        VB 
+          (VBBExpBinOp 
+            (op \<and>) 
+            (VBBVarOp FMon)
+            (VBBExpUnOp Not (VBBConstOp (P (VBVVarOp (MonIn 1))))))
+          (VBVVarOp (MonIn 1))
       ])
     }))"
 
-definition SMon :: "(FailureVarName \<Rightarrow> bool) \<Rightarrow> (ValueVarName \<Rightarrow> Values) \<Rightarrow> (FailureVarName, ValueVarName) System" where
-  "SMon val_b val_v\<equiv> (
+fun option_op :: "('a \<Rightarrow> 'a \<Rightarrow> bool) \<Rightarrow> 'a option \<Rightarrow> 'a option \<Rightarrow> bool" where
+  "option_op f None vo = False" |
+  "option_op f vo None = False" |
+  "option_op f (Some v1) (Some v2) = f v1 v2"
+
+fun lt_values :: "Values \<Rightarrow> Values \<Rightarrow> bool" where
+  "lt_values (FMFailure f) v = True" |
+  "lt_values v (FMFailure f) = False" |
+  "lt_values (FMNominal n1) (FMNominal n2) = (n1 \<le> n2)"
+
+definition SMon :: "(FailureVarName \<Rightarrow> bool) \<Rightarrow> (ValueVarName \<Rightarrow> Values) \<Rightarrow> 
+    (FailureVarName, ValueVarName) System" where
+  "SMon vb vv \<equiv> (
     {
       Battery 1, Battery 2, 
-      Monitor 3 (\<lambda> Es. ((ValuedBoolExp_value_eval Es val_b val_v) = (FMNominal 2)))
+      Monitor 3 (\<lambda> Es. option_op lt_values (Some (FMNominal 2)) (ValuesOperand_value_eval Es vb vv))
     }, 
     {((1,1), (3,1)), ((2,1), (3,2))}
   )"
